src/Bedrock/Proofs/ValidComputable.v
@@ -1,0 +1,1620 @@
+Require Import Coq.ZArith.ZArith.
+Require Import Coq.Bool.Bool.
+Require Import Coq.Lists.List.
+Require Import Coq.micromega.Lia.
+Require Import bedrock2.Syntax.
+Require Import coqutil.Word.Interface coqutil.Word.Properties.
+Require Import coqutil.Map.Interface.
+Require Import Crypto.Bedrock.Types.
+Require Import Crypto.Bedrock.Translation.Expr.
+Require Import Crypto.Bedrock.Proofs.Expr.
+Require Import Crypto.Language.API.
+Require Import Crypto.Util.Decidable.
+Require Import Crypto.Util.ZRange.
+Require Import Crypto.Util.Tactics.BreakMatch.
+Require Import Crypto.Util.ZUtil.Tactics.LtbToLt.
+Require Import Crypto.Util.Bool.Reflect.
+Local Open Scope Z_scope.
+Local Open Scope bool_scope.
+
+Import API.Compilers.
+Import Wf.Compilers.expr.
+Import Types.Notations Types.Types.
+
+Section Expr.
+  Context {p : Types.parameters} {p_ok : @ok p}.
+
+  Local Existing Instance Types.rep.Z.
+  Local Existing Instance Types.rep.listZ_local.
+  Local Instance sem_ok : Semantics.parameters_ok semantics
+    := semantics_ok.
+
+  Definition is_fst_snd_ident {t} (i : ident.ident t) : bool :=
+    match i with
+    | ident.fst base_Z base_Z => true
+    | ident.snd base_Z base_Z => true
+    | _ => false
+    end.
+
+  Definition valid_expr_App1_bool {t} (require_casts : bool)
+           (e : @API.expr (fun _ => unit) t) : bool :=
+    match e with
+    | expr.App type_range (type.arrow type_Z type_Z) f r =>
+      is_cast_ident_expr f && is_cast_literal r
+    | expr.App type_range2 (type.arrow type_ZZ type_ZZ) f r =>
+      is_cast_ident_expr f && is_cast2_literal r
+    | expr.Ident (type.arrow type_ZZ type_Z) i =>
+      negb require_casts && is_fst_snd_ident i
+    | _ => false
+    end.
+
+  Definition is_mul_high_ident {t} (i : ident.ident t) : bool :=
+    match i with
+    | ident.Z_mul_high => true
+    | _ => false
+    end.
+  Definition is_mul_high_ident_expr {t}
+           (e : @API.expr (fun _ => unit) t) : bool :=
+    match e with
+    | expr.Ident (type.arrow type_Z
+                             (type.arrow type_Z
+                                         (type.arrow type_Z type_Z)))
+                 i => is_mul_high_ident i
+    | _ => false
+    end.
+  
+  Definition valid_expr_App2_bool {t} (require_casts : bool)
+           (e : @API.expr (fun _ => unit) t) : bool :=
+    match e with
+    | expr.App
+        type_Z (type.arrow type_Z (type.arrow type_Z type_Z))
+        f (expr.Ident _ (ident.Literal base.type.Z s)) =>
+      (is_mul_high_ident_expr f)
+        && (negb require_casts)
+        && (Z.eqb s (2 ^ Semantics.width))
+    | expr.Ident (type.arrow type_Z (type.arrow type_Z type_Z)) i =>
+      match translate_binop i with
+      | None => false
+      | Some _ => negb require_casts
+      end
+    | _ => false
+    end.
+
+  Definition is_shiftl_ident {t} (i : ident.ident t) :=
+    match i with
+    | ident.Z_truncating_shiftl => true
+    | _ => false
+    end.
+  Definition is_shiftl_ident_expr 
+             {t} (e : @API.expr (fun _ => unit) t) :=
+    match e with
+    | expr.Ident
+        (type.arrow type_Z (type.arrow type_Z (type.arrow type_Z type_Z)))
+        i => is_shiftl_ident i
+    | _ => false
+    end.
+  Definition valid_expr_shift_bool {t} (require_casts : bool)
+           (e : @API.expr (fun _ => unit) t) : bool :=
+    match e with
+    | expr.App
+        type_Z (type.arrow type_Z (type.arrow type_Z type_Z))
+        f (expr.Ident _ (ident.Literal base.type.Z s)) =>
+      (is_shiftl_ident_expr f)
+        && (negb require_casts)
+        && Z.eqb s Semantics.width
+    | expr.Ident _ ident.Z_shiftr =>
+      negb require_casts
+    | _ => false
+    end.
+
+  Definition valid_shifter {t}
+           (e : @API.expr (fun _ => unit) t) : bool :=
+    match e with
+    | expr.Ident _ (ident.Literal base.type.Z n) =>
+      is_bounded_by_bool n width_range
+    | _ => false
+    end.
+
+  Definition valid_expr_nth_default_App3_bool {t}
+           (e : @API.expr (fun _ => unit) t) : bool :=
+    match e with
+    | expr.Ident _ (ident.List_nth_default base_Z) =>
+      true
+    | _ => false
+    end.
+  Definition valid_expr_nth_default_App2_bool {t}
+           (e : @API.expr (fun _ => unit) t) : bool :=
+    match e with
+    | expr.App
+        type_Z (type.arrow
+                  type_listZ
+                  (type.arrow type_nat type_Z))
+        f (expr.Ident _ (ident.Literal base.type.Z d)) =>
+      valid_expr_nth_default_App3_bool f && is_bounded_by_bool d max_range
+    | _ => false
+    end.
+  Definition valid_expr_nth_default_App1_bool {t}
+           (e : @API.expr (fun _ => unit) t) : bool :=
+    match e with
+    | expr.App type_listZ (type.arrow type_nat type_Z)
+               f (expr.Var _ l) =>
+      valid_expr_nth_default_App2_bool f
+    | _ => false
+    end.
+  Definition valid_expr_nth_default_bool {t}
+           (e : @API.expr (fun _ => unit) t) : bool :=
+    match e with
+    | expr.App
+        type_nat type_Z
+        f (expr.Ident _ (ident.Literal base.type.nat i)) =>
+      valid_expr_nth_default_App1_bool f
+    | _ => false
+    end.
+
+  Fixpoint valid_expr_bool {t} (require_casts : bool)
+             (e : @API.expr (fun _ => unit) t) {struct e} : bool :=
+    match e with
+    | expr.App type_nat _ f x =>
+      (* only thing accepting nat is nth_default *)
+      if require_casts
+      then false
+      else valid_expr_nth_default_bool (expr.App f x)
+    | expr.App type_Z type_Z
+               (expr.App type_Z _ f x) y =>
+      if valid_expr_App2_bool require_casts f
+      then valid_expr_bool true x && valid_expr_bool true y
+      else if valid_expr_shift_bool require_casts f
+           then valid_expr_bool true x && valid_shifter y
+           else false
+    | expr.App type_Z type_Z f x =>
+      valid_expr_App1_bool require_casts f && valid_expr_bool true x
+    | expr.App type_ZZ type_Z f x =>
+      valid_expr_App1_bool require_casts f && valid_expr_bool true x
+    | expr.App type_ZZ type_ZZ f x =>
+      valid_expr_App1_bool require_casts f && valid_expr_bool true x
+    | expr.Ident _ (ident.Literal base.type.Z z) =>
+      negb require_casts || is_bounded_by_bool z max_range
+    | expr.Ident _ (ident.Literal base.type.nat n) =>
+      negb require_casts
+    | expr.Var type_Z v => negb require_casts
+    | expr.Var type_listZ v => true
+    | _ => false
+    end.
+ 
+  Lemma valid_expr_App1_bool_type {t} rc (e : API.expr t) :
+    valid_expr_App1_bool rc e = true ->
+    (exists d,
+        t = type.arrow type_Z d
+        \/ t = type.arrow type_ZZ d).
+  Proof.
+    cbv [valid_expr_App1_bool].
+    destruct e;
+      match goal with
+      | idc : ident.ident _ |- _ =>
+        destruct idc; try congruence;
+          break_match; try congruence; intros;
+            eexists; right; reflexivity
+      | v: unit, t : API.type |- _ =>
+        destruct t; congruence
+      | f : API.expr (?s -> ?d) |- _ =>
+        destruct d;
+          break_match; try congruence;
+        try (eexists; right; reflexivity);
+        eexists; left; reflexivity
+      | |- forall (_: false = true), _ => congruence
+      | |- context [@expr.LetIn _ _ _ _ ?B] =>
+        destruct B; congruence
+      | _ => idtac
+      end.
+  Qed.
+
+  Lemma is_mul_high_ident_expr_type {t} (f : API.expr t) :
+    is_mul_high_ident_expr f = true ->
+    t = type.arrow type_Z
+                   (type.arrow type_Z
+                               (type.arrow type_Z type_Z)).
+  Proof.
+    cbv [is_mul_high_ident_expr].
+    break_match; congruence.
+  Qed.
+
+  Lemma valid_expr_shift_bool_type {t} rc (f : API.expr t) :
+    valid_expr_shift_bool rc f = true ->
+    t = type.arrow type_Z
+                   (type.arrow type_Z type_Z).
+  Proof.
+    cbv [valid_expr_shift_bool].
+    break_match; congruence.
+  Qed.
+
+  Lemma valid_expr_App2_bool_type {t} rc (f : API.expr t) :
+    valid_expr_App2_bool rc f = true ->
+    t = type.arrow type_Z
+                   (type.arrow type_Z type_Z).
+  Proof.
+    cbv [valid_expr_App2_bool translate_binop].
+    destruct f;
+      match goal with
+      | idc : ident.ident _ |- _ =>
+        destruct idc; try congruence;
+          break_match; congruence
+      | |- forall (_: false = true), _ => congruence
+      | _ => idtac
+      end; [ ].
+    break_match; congruence.
+  Qed.
+
+  Lemma valid_expr_nth_default_App2_bool_type {t}
+        (f : API.expr t) :
+    valid_expr_nth_default_App2_bool f = true ->
+    match t with
+    | type.arrow type_listZ
+                 (type.arrow type_nat type_Z) =>
+      True
+    | _ => False
+    end.
+  Proof.
+    cbv [valid_expr_nth_default_App2_bool].
+    break_match; try congruence; [ ].
+    tauto.
+  Qed.
+
+  Lemma valid_expr_nth_default_App1_bool_type {t}
+        (f : API.expr t) :
+    valid_expr_nth_default_App1_bool f = true ->
+    match t with
+    | type.arrow type_nat type_Z =>
+      True
+    | _ => False
+    end.
+  Proof.
+    cbv [valid_expr_nth_default_App1_bool].
+    break_match; try congruence; [ ].
+    tauto.
+  Qed.
+
+  Lemma valid_expr_nth_default_App3_bool_impl1 {t}
+        (f : API.expr t) n l d :
+    valid_expr_nth_default_App3_bool f = true ->
+    is_bounded_by_bool d max_range = true ->
+    (match t as t0 return expr.expr t0 -> Prop with
+     | type.arrow type_Z
+                  (type.arrow type_listZ (type.arrow type_nat type_Z)) =>
+       fun f =>
+         valid_expr
+           false (expr.App
+                    (expr.App
+                       (expr.App
+                          f
+                          (expr.Ident
+                             (ident.Literal (t:=base.type.Z) d)))
+                       (expr.Var l))
+                 (expr.Ident (ident.Literal (t:=base.type.nat) n)))
+     | _ => fun _ => False
+     end) f.
+  Proof.
+    cbv [valid_expr_nth_default_App3_bool].
+    break_match; try congruence; [ ].
+    intros. constructor.
+    cbv [is_bounded_by_bool upper lower max_range] in *.
+    repeat match goal with
+           | H : _ && _ = true |- _ =>
+             apply andb_true_iff in H; destruct H
+           end.
+    Z.ltb_to_lt; lia.
+  Qed.
+
+  Lemma valid_expr_nth_default_App2_bool_impl1 {t}
+        (f : API.expr t) n l :
+    valid_expr_nth_default_App2_bool f = true ->
+    (match t as t0 return expr.expr t0 -> Prop with
+     | type.arrow type_listZ (type.arrow type_nat type_Z) =>
+       fun f =>
+         valid_expr
+           false
+           (expr.App
+              (expr.App f (expr.Var l))
+              (expr.Ident (ident.Literal (t:=base.type.nat) n)))
+     | _ => fun _ => False
+     end) f.
+  Proof.
+    cbv [valid_expr_nth_default_App2_bool].
+    break_match; try congruence; [ ].
+    intros;
+      repeat match goal with
+             | H : _ && _ = true |- _ =>
+               apply andb_true_iff in H; destruct H
+             | H : valid_expr_nth_default_App3_bool _ = true |- _ =>
+               eapply valid_expr_nth_default_App3_bool_impl1 in H;
+                 eassumption
+             end.
+  Qed.
+
+  Lemma valid_expr_nth_default_App1_bool_impl1 {t}
+        (f : API.expr t) n :
+    valid_expr_nth_default_App1_bool f = true ->
+    (match t as t0 return expr.expr t0 -> Prop with
+     | type.arrow type_nat type_Z =>
+       fun f =>
+         valid_expr
+           false (expr.App f
+                        (expr.Ident (ident.Literal (t:=base.type.nat) n)))
+     | _ => fun _ => False
+     end) f.
+  Proof.
+    cbv [valid_expr_nth_default_App1_bool].
+    break_match; try congruence; [ ].
+    intros;
+      repeat match goal with
+             | H : _ && _ = true |- _ =>
+               apply andb_true_iff in H; destruct H
+             end;
+      match goal with
+      | H : valid_expr_nth_default_App2_bool _ = true |- _ =>
+        eapply valid_expr_nth_default_App2_bool_impl1 in H
+      end.
+    break_match_hyps; try tauto; [ ].
+    eassumption.
+  Qed.
+
+  Lemma is_fst_snd_ident_impl1 {t} (i : ident.ident t) :
+    is_fst_snd_ident i = true ->
+    (match t as t0 return ident.ident t0 -> Prop with
+     | type.arrow type_ZZ type_Z =>
+       fun i =>
+         forall x : API.expr type_ZZ,
+           valid_expr true x ->
+           valid_expr false (expr.App (expr.Ident i) x)
+     | _ => fun _ => False
+     end) i.
+  Proof.
+    cbv [is_fst_snd_ident].
+    break_match; try congruence; [ | ];
+      intros; constructor; eauto.
+  Qed.
+
+  Lemma is_cast_literal_ident_eq {t} (i : ident.ident t) :
+    is_cast_literal_ident i = true ->
+    (match t as t0 return ident.ident t0 -> Prop with
+     | type_range =>
+       fun i => i = ident.Literal (t:=base.type.zrange) max_range
+     | _ => fun _ => False
+     end) i.
+  Proof.
+    cbv [is_cast_literal_ident].
+    break_match; try congruence; [ ].
+    cbv [range_good].
+    intros; progress reflect_beq_to_eq zrange_beq; subst.
+    reflexivity.
+  Qed.
+
+  Lemma is_cast_literal_eq {t} (r : API.expr t) :
+    is_cast_literal r = true ->
+    (match t as t0 return @API.expr (fun _ => unit) t0 -> Prop with
+     | type_range =>
+       fun r =>
+         r = expr.Ident (ident.Literal (t:=base.type.zrange) max_range)
+     | _ => fun _ => False
+     end) r.
+  Proof.
+    cbv [is_cast_literal].
+    break_match; try congruence; [ ].
+    intros;
+      match goal with
+      | H : is_cast_literal_ident _ = true |- _ =>
+        apply is_cast_literal_ident_eq in H
+      end.
+    congruence.
+  Qed.
+
+  Lemma is_pair_range_eq {t} (i : ident.ident t) :
+    is_pair_range i = true ->
+    (match t as t0 return ident.ident t0 -> Prop with
+     | type.arrow type_range (type.arrow type_range type_range2) =>
+       fun i => i = ident.pair
+     | _ => fun _ => False
+     end) i.
+  Proof.
+    cbv [is_pair_range].
+    break_match; congruence.
+  Qed.
+
+  Lemma is_cast2_literal_App2_eq {t} (r : API.expr t) :
+    is_cast2_literal_App2 r = true ->
+    (match t as t0 return @API.expr (fun _ => unit) t0 -> Prop with
+     | type.arrow type_range (type.arrow type_range type_range2) =>
+       fun r => r = expr.Ident ident.pair
+     | _ => fun _ => False
+     end) r.
+  Proof.
+    cbv [is_cast2_literal_App2].
+    break_match; try congruence; [ ].
+    intros;
+      match goal with
+      | H : is_pair_range _ = true |- _ =>
+        apply is_pair_range_eq in H
+      end.
+    congruence.
+  Qed.
+
+  Lemma is_cast2_literal_App1_eq {t} (r : API.expr t) :
+    is_cast2_literal_App1 r = true ->
+    (match t as t0 return @API.expr (fun _ => unit) t0 -> Prop with
+     | type.arrow type_range type_range2 =>
+       fun r =>
+         r = expr.App
+               (expr.Ident ident.pair)
+               (expr.Ident
+                  (ident.Literal (t:=base.type.zrange) max_range))
+     | _ => fun _ => False
+     end) r.
+  Proof.
+    cbv [is_cast2_literal_App1].
+    break_match; try congruence; [ ].
+    intros;
+      repeat match goal with
+             | H : _ && _ = true |- _ =>
+               apply andb_true_iff in H; destruct H
+             | H : is_cast_literal _ = true |- _ =>
+               apply is_cast_literal_eq in H; subst
+             | H : is_cast2_literal_App2 _ = true |- _ =>
+               apply is_cast2_literal_App2_eq in H; subst
+             end.
+    congruence.
+  Qed.
+
+  Lemma is_cast2_literal_eq {t} (r : API.expr t) :
+    is_cast2_literal r = true ->
+    (match t as t0 return @API.expr (fun _ => unit) t0 -> Prop with
+     | type_range2 =>
+       fun r =>
+         r = expr.App
+               (expr.App
+                  (expr.Ident ident.pair)
+                  (expr.Ident
+                     (ident.Literal (t:=base.type.zrange) max_range)))
+               (expr.Ident
+                  (ident.Literal (t:=base.type.zrange) max_range))
+     | _ => fun _ => False
+     end) r.
+  Proof.
+    cbv [is_cast2_literal].
+    break_match; try congruence; [ ].
+    intros;
+      repeat match goal with
+             | H : _ && _ = true |- _ =>
+               apply andb_true_iff in H; destruct H
+             | H : is_cast_literal _ = true |- _ =>
+               apply is_cast_literal_eq in H; subst
+             | H : is_cast2_literal_App1 _ = true |- _ =>
+               apply is_cast2_literal_App1_eq in H; subst
+             end.
+    congruence.
+  Qed.
+
+  Lemma is_cast_ident_expr_impl1 {t} rc (f : API.expr t) :
+    is_cast_ident_expr f = true ->
+    (match t as t0 return expr.expr t0 -> Prop with
+     | type.arrow type_range (type.arrow type_Z type_Z) =>
+       fun f =>
+         forall
+           (r : API.expr type_range)
+           (x : API.expr type_Z),
+           is_cast_literal r = true ->
+           valid_expr false x ->
+           valid_expr rc (expr.App (expr.App f r) x)
+     | type.arrow type_range2 (type.arrow type_ZZ type_ZZ) =>
+       fun f =>
+         forall
+           (r : API.expr type_range2)
+           (x : API.expr type_ZZ),
+           is_cast2_literal r = true ->
+           valid_expr false x ->
+           valid_expr rc (expr.App (expr.App f r) x)
+     | _ => fun _ => False
+     end) f.
+  Proof.
+    cbv [is_cast_ident_expr is_cast_ident].
+    break_match; try congruence; [ | ];
+      intros;
+      match goal with
+      | H : is_cast_literal _ = true |- _ =>
+        apply is_cast_literal_eq in H; subst
+      | H : is_cast2_literal _ = true |- _ =>
+        apply is_cast2_literal_eq in H; subst
+      end.
+    { constructor;
+        cbv [range_good]; auto using zrange_lb. }
+    { constructor;
+        cbv [range_good]; auto using zrange_lb. }
+  Qed.
+
+  Lemma valid_expr_App1_bool_impl1 {t}
+        rc (f : API.expr t) :
+    valid_expr_App1_bool rc f = true ->
+    (match t as t0 return expr.expr t0 -> Prop with
+     | type.arrow type_Z _ =>
+       fun f =>
+         forall x : API.expr type_Z,
+           valid_expr false x ->
+           valid_expr rc (expr.App f x)
+     | type.arrow type_ZZ type_Z =>
+       fun f =>
+         forall x : API.expr type_ZZ,
+           valid_expr true x ->
+           valid_expr rc (expr.App f x)
+     | type.arrow type_ZZ type_ZZ =>
+       fun f =>
+         forall x : API.expr type_ZZ,
+           valid_expr false x ->
+           valid_expr rc (expr.App f x)
+     | _ => fun _ => False
+     end) f.
+  Proof.
+    cbv [valid_expr_App1_bool].
+    remember t.
+    destruct t; try congruence.
+    { intros; exfalso.
+      break_match_hyps; congruence. }
+    { break_match; try congruence; [ | | ]; intros;
+        repeat match goal with
+               | H : _ && _ = true |- _ =>
+                 apply andb_true_iff in H; destruct H
+               | H : negb ?rc = true |- _ =>
+                 destruct rc; cbn [negb] in *; try congruence; [ ]
+               | H : is_fst_snd_ident _ = true |- _ =>
+                 apply is_fst_snd_ident_impl1 in H; solve [eauto]
+               | H : is_cast_ident_expr _ = true |- _ =>
+                 eapply is_cast_ident_expr_impl1 in H;
+                   apply H; solve [eauto]
+               end. }
+  Qed.
+
+  Lemma valid_expr_nth_default_bool_impl1 {t}
+        (e : API.expr t) :
+    (exists b, t = type.base b) ->
+    valid_expr_nth_default_bool e = true ->
+    valid_expr false e.
+  Proof.
+    cbv [valid_expr_nth_default_bool].
+    intro; destruct e; try congruence; [ ].
+    match goal with
+      | _ : API.expr (type.arrow _ ?d) |- _ =>
+        destruct d
+    end;
+      break_match; try congruence; intros; [ ].
+    match goal with
+    | H : valid_expr_nth_default_App1_bool _ = true |- _ =>
+      eapply valid_expr_nth_default_App1_bool_impl1 in H
+    end.
+    eassumption.
+  Qed.
+
+  Lemma is_mul_high_ident_eq {t} (i : ident.ident t) :
+    is_mul_high_ident i = true ->
+    (match t as t0 return ident.ident t0 -> Prop with
+     | type.arrow type_Z (type.arrow type_Z (type.arrow type_Z type_Z)) =>
+       fun i => i = ident.Z_mul_high
+     | _ => fun _ => False
+     end) i.
+  Proof.
+    cbv [is_mul_high_ident].
+    break_match; congruence.
+  Qed.
+
+  Lemma is_mul_high_ident_expr_eq {t} (f : API.expr t) :
+    is_mul_high_ident_expr f = true ->
+    (match t as t0 return API.expr t0 -> Prop with
+     | type.arrow type_Z (type.arrow type_Z (type.arrow type_Z type_Z)) =>
+       fun f => f = expr.Ident ident.Z_mul_high
+     | _ => fun _ => False
+     end) f.
+  Proof.
+    cbv [is_mul_high_ident_expr].
+    break_match; try congruence; [ ].
+    intros;
+      match goal with
+      | H : is_mul_high_ident _ = true |- _ =>
+        apply is_mul_high_ident_eq in H
+      end.
+    congruence.
+  Qed.
+
+  Lemma valid_expr_App2_bool_impl1 {t}
+        rc (f : API.expr t) :
+    valid_expr_App2_bool rc f = true ->
+    (match t as t0 return expr.expr t0 -> Prop with
+     | type.arrow type_Z (type.arrow type_Z type_Z) =>
+       fun f =>
+         forall x y : API.expr type_Z,
+           valid_expr true x ->
+           valid_expr true y ->
+           valid_expr rc (expr.App (expr.App f x) y)
+     | _ => fun _ => False
+     end) f.
+  Proof.
+    cbv [valid_expr_App2_bool].
+    break_match; try congruence; [ | ];
+      intros;
+      repeat match goal with
+             | H : _ && _ = true |- _ =>
+               apply andb_true_iff in H; destruct H
+             | H : negb ?rc = true |- _ =>
+               destruct rc; cbn [negb] in *; try congruence; [ ]
+             | H : is_mul_high_ident_expr _ = true |- _ =>
+               apply is_mul_high_ident_expr_eq in H; subst
+             end; [ | ].
+    { constructor; eauto; congruence. }
+    { constructor; eauto; Z.ltb_to_lt; congruence. }
+  Qed.
+
+  Lemma is_shiftl_ident_eq {t} (i : ident.ident t) :
+    is_shiftl_ident i = true ->
+    (match t as t0 return ident.ident t0 -> Prop with
+     | type.arrow type_Z (type.arrow type_Z (type.arrow type_Z type_Z)) =>
+       fun i => i = ident.Z_truncating_shiftl
+     | _ => fun _ => False
+     end) i.
+  Proof.
+    cbv [is_shiftl_ident].
+    break_match; congruence.
+  Qed.
+
+  Lemma is_shiftl_ident_expr_eq {t} (f : API.expr t) :
+    is_shiftl_ident_expr f = true ->
+    (match t as t0 return API.expr t0 -> Prop with
+     | type.arrow type_Z (type.arrow type_Z (type.arrow type_Z type_Z)) =>
+       fun f => f = expr.Ident ident.Z_truncating_shiftl
+     | _ => fun _ => False
+     end) f.
+  Proof.
+    cbv [is_shiftl_ident_expr].
+    break_match; try congruence; [ ].
+    intros;
+      match goal with
+      | H : is_shiftl_ident _ = true |- _ =>
+        apply is_shiftl_ident_eq in H
+      end.
+    congruence.
+  Qed.
+
+  Lemma valid_shifter_eq {t} (x : API.expr t) :
+    valid_shifter x = true ->
+    (match t as t0 return expr.expr t0 -> Prop with
+     | type_Z =>
+       fun x =>
+         exists n,
+           is_bounded_by_bool n width_range = true /\
+           x = expr.Ident (ident.Literal (t:=base.type.Z) n)
+     | _ => fun _ => False
+     end) x.
+  Proof.
+    cbv [valid_shifter].
+    break_match; try congruence; [ ].
+    intros; eexists; eauto.
+  Qed.
+
+  Lemma valid_expr_shift_bool_impl1 {t}
+        rc (f : API.expr t) :
+    valid_expr_shift_bool rc f = true ->
+    (match t as t0 return expr.expr t0 -> Prop with
+     | type.arrow type_Z (type.arrow type_Z type_Z) =>
+       fun f =>
+         forall x y : API.expr type_Z,
+           valid_expr true x ->
+           valid_shifter y = true ->
+           valid_expr rc (expr.App (expr.App f x) y)
+     | _ => fun _ => False
+     end) f.
+  Proof.
+    cbv [valid_expr_shift_bool].
+    break_match; try congruence; [ | ];
+      intros;
+      repeat match goal with
+             | H : _ && _ = true |- _ =>
+               apply andb_true_iff in H; destruct H
+             | H : negb ?rc = true |- _ =>
+               destruct rc; cbn [negb] in *; try congruence; [ ]
+             | H : is_bounded_by_bool _ width_range = true |- _ =>
+               cbv [is_bounded_by_bool upper lower width_range] in H
+             | H : is_shiftl_ident_expr _ = true |- _ =>
+               apply is_shiftl_ident_expr_eq in H; subst
+             | H : valid_shifter _ = true |- _ =>
+               apply valid_shifter_eq in H;
+                 destruct H as [? [? ?] ]; subst
+             end.
+    { Z.ltb_to_lt.
+      constructor; eauto; lia. }
+    { Z.ltb_to_lt.
+      constructor; eauto; lia. }
+  Qed.
+
+  Lemma valid_expr_App_bool_impl1 {t} rc
+        (f : API.expr t) (y : API.expr type_Z) :
+    match f with
+    | expr.App type_Z _ f x =>
+      if valid_expr_App2_bool rc f
+      then valid_expr_bool true x && valid_expr_bool true y
+      else if valid_expr_shift_bool rc f
+           then valid_expr_bool true x && valid_shifter y
+           else false
+    | _ => false
+    end = true ->
+    (match t as t0 return expr.expr t0 -> Prop with
+     | type.arrow type_Z type_Z =>
+       fun f =>
+           valid_expr true y ->
+           valid_expr rc (expr.App f y)
+     | type.arrow type_ZZ _ =>
+       fun f =>
+         forall y,
+           valid_expr true y ->
+           valid_expr rc (expr.App f y)
+     | _ => fun _ => False
+     end) f.
+  Proof.
+    intro. remember t.
+    break_match;
+      try match goal with
+          | |- forall (_:false = true), _ => congruence
+          | H : valid_expr_App2_bool _ _ = true |- _ =>
+            apply valid_expr_App2_bool_type in H;
+              congruence
+          | H : valid_expr_shift_bool _ _ = true |- _ =>
+            apply valid_expr_shift_bool_type in H;
+              congruence
+          end; [ | ].
+    { intros;
+        repeat match goal with
+               | H : _ && _ = true |- _ =>
+                 apply andb_true_iff in H; destruct H
+               | H : valid_expr_App2_bool _ _ = true |- _ =>
+                 apply valid_expr_App2_bool_impl1 in H
+               end.
+      eauto. }
+    { intros; 
+        repeat match goal with
+               | H : _ && _ = true |- _ =>
+                 apply andb_true_iff in H; destruct H
+               | H : valid_expr_shift_bool _ _ = true |- _ =>
+                 apply valid_expr_shift_bool_impl1 in H
+               end.
+      eauto. }
+  Qed.
+
+  Lemma valid_expr_bool_impl1 {t} (e : API.expr t) :
+    (exists b, t = type.base b) ->
+    forall rc,
+      valid_expr_bool rc e = true -> valid_expr rc e.
+  Proof.
+    induction e; intros;
+      cbn [valid_expr_bool] in *.
+    { break_match_hyps; try congruence.
+      { constructor.
+        repeat match goal with
+               | _ => progress cbn [orb]
+               | H : _ || _ = true |- _ =>
+                 apply orb_true_iff in H; destruct H
+               | H : _ = true |- _ => rewrite H
+               | _ => rewrite Bool.orb_true_r
+               | _ => reflexivity
+               end. }
+      { destruct rc; cbn [negb] in *; try congruence.
+        constructor. } }
+    { break_match_hyps; try congruence.
+      { destruct rc; cbn [negb] in *; try congruence.
+        constructor. }
+      { constructor. } }
+    { break_match_hyps; congruence. }
+    { remember s.
+      break_match_hyps; try congruence;
+          repeat match goal with
+                 | H : _ && _ = true |- _ =>
+                   apply andb_true_iff in H; destruct H
+                 | H: valid_expr_App1_bool _ _ = true |- _ =>
+                   apply valid_expr_App1_bool_type in H;
+                     destruct H; destruct H; congruence
+                 end; [ | | | ].
+      { apply (@valid_expr_App_bool_impl1 (type.arrow type_Z type_Z)).
+        { 
+        break_match; try congruence;
+          repeat match goal with
+                 | H : _ && _ = true |- _ =>
+                   apply andb_true_iff in H; destruct H
+                 | _ => assumption
+                 end. }
+      { eauto using valid_expr_nth_default_bool_impl1. }
+      { pose proof H0.
+        apply valid_expr_App1_bool_type in H0.
+        destruct H0. destruct H0; try congruence.
+        inversion H0; subst.
+        (* need valid_expr_App1_bool_impl1 like nth_default model *)
+        (* probably get rid of current valid_expr_App_bool_impl1? *)
+
+  Fixpoint valid_expr_bool {t} (require_casts : bool)
+             (e : @API.expr (fun _ => unit) t) : bool :=
+    match e with
+    | expr.App
+        (expr.Ident _ (ident.Literal base.type.zrange r))) x =>
+      range_good r && valid_expr_bool false x
+    | expr.App
+        _ _
+        (expr.App
+           _ _ (expr.Ident _ ident.Z_cast2)
+           (expr.App
+              _ _
+              (expr.App
+                 _ _
+                 (expr.Ident _ (ident.pair _ _))
+                 (expr.Ident _ (ident.Literal base.type.zrange r1)))
+              (expr.Ident _ (ident.Literal base.type.zrange r2)))) x =>
+      range_good r1 && range_good r2 && valid_expr_bool false x
+    | expr.App _ _ (expr.Ident _ (ident.fst _ _)) x =>
+      negb require_casts && valid_expr_bool true x
+    | expr.App _ _ (expr.Ident _ (ident.snd _ _)) x =>
+      negb require_casts && valid_expr_bool true x
+    | expr.Ident _ (ident.Literal base.type.Z z) =>
+      negb require_casts || is_bounded_by_bool z max_range
+    | expr.Ident _ (ident.Literal base.type.nat n) =>
+      negb require_casts
+    | expr.Var type_Z v => negb require_casts
+    | expr.Var type_listZ v => true
+    | expr.App
+        _ _ (expr.App
+               _ _ (expr.App
+                      _ _ (expr.Ident _ (ident.List_nth_default _)) d)
+               (expr.Var type_listZ l))
+        (expr.Ident _ (ident.Literal base.type.nat i)) =>
+      negb require_casts && valid_expr_bool true d
+    | expr.App
+        _ _ (expr.App
+               _ _ (expr.Ident _ ident.Z_shiftr) x)
+        (expr.Ident _ (ident.Literal base.type.Z n)) =>
+      negb require_casts && is_bounded_by_bool n width_range
+           && valid_expr_bool true x
+    | expr.App
+        _ _ (expr.App
+               _ _ (expr.App
+                      _ _ (expr.Ident _ ident.Z_mul_high)
+                      (expr.Ident _ (ident.Literal base.type.Z s)))
+               x) y =>
+      negb require_casts && Z.eqb s (2 ^ Semantics.width)
+           && valid_expr_bool true x && valid_expr_bool true y
+    | expr.App
+        _ _ (expr.App
+               _ _ (expr.App
+                      _ _ (expr.Ident _ ident.Z_truncating_shiftl)
+                      (expr.Ident _ (ident.Literal base.type.Z s)))
+               x)
+        (expr.Ident _ (ident.Literal base.type.Z n)) =>
+      negb require_casts && is_bounded_by_bool n width_range
+           && Z.eqb s Semantics.width && valid_expr_bool true x
+    | expr.App
+        _ _ (expr.App _ _ (expr.Ident _ i) x) y =>
+      match translate_binop i with
+      | None => false
+      | Some _ =>
+        negb require_casts && valid_expr_bool true x
+             && valid_expr_bool true y
+      end
+    | _ => false
+    end.
+  (* TODO: remove nat case *)
+
+
+  Lemma valid_expr_bool_impl1 {t} (e : API.expr t) :
+    forall rc,
+      valid_expr_bool rc e = true -> valid_expr rc e.
+  Proof.
+    induction e; intros;
+      cbn [valid_expr_bool] in *.
+    { break_match_hyps; try congruence.
+      { constructor.
+        repeat match goal with
+               | _ => progress cbn [orb]
+               | H : _ || _ = true |- _ =>
+                 apply orb_true_iff in H; destruct H
+               | H : _ = true |- _ => rewrite H
+               | _ => rewrite Bool.orb_true_r
+               | _ => reflexivity
+               end. }
+      { destruct rc; cbn [negb] in *; try congruence.
+        constructor. } }
+    { break_match_hyps; try congruence.
+      { destruct rc; cbn [negb] in *; try congruence.
+        constructor. }
+      { constructor. } }
+    { break_match_hyps; try congruence. }
+    { break_match_hyps; try congruence.
+        repeat match goal with
+               | _ => progress cbn [orb]
+               | H : _ || _ = true |- _ =>
+                 apply orb_true_iff in H; destruct H
+               | H : _ = true |- _ => rewrite H
+               | _ => rewrite Bool.orb_true_r
+               | _ => reflexivity
+               end.
+        
+        
+        
+      cbn [valid_expr_bool cast_exempt negb andb] in *;
+      break_match_hyps;
+      cbn [valid_ident_bool valid_cast_exempt_bool
+                            valid_cast_bool
+                            translate_binop] in *;
+      repeat match goal with
+             | H : false = true |- _ => congruence
+             | H : true = false |- _ => congruence
+             | H : exists _, type.arrow _ _ = type.base _ |- _ =>
+               destruct H; congruence
+             | _ => progress subst
+             | H : _ && _ = true |- _ =>
+               apply andb_true_iff in H; destruct H
+             | H : _ && _ = false |- _ =>
+               apply andb_false_iff in H; destruct H
+             end.
+
+  Definition valid_ident_bool {t} (i : ident.ident t)
+    : type.for_each_lhs_of_arrow API.expr t -> (* argument expressions *)
+      bool :=
+    match i in ident.ident t0 return
+          type.for_each_lhs_of_arrow (@API.expr (fun _ => unit))
+                                     t0 -> bool with
+    | ident.fst _ _ => fun _ => true
+    | ident.snd _ _ => fun _ => true
+    | ident.Z_cast => fun _ => true
+    | ident.Z_cast2 => fun _ => true
+    | ident.List_nth_default base_Z =>
+      fun args =>
+        let '(d, (l, (i, _))) := args in
+        match i with
+        | expr.Ident _ (ident.Literal base.type.nat i) =>
+          true
+        | _ => false
+        end
+    | ident.Z_shiftr =>
+      fun args =>
+        let '(x, (n, _)) := args in
+        match n with
+        | expr.Ident _ (ident.Literal base.type.Z n) =>
+          is_bounded_by_bool n width_range
+        | _ => false
+        end
+    | ident.Z_truncating_shiftl =>
+      fun args =>
+        let '(s, (x, (n, _))) := args in
+        match s with
+        | expr.Ident _ (ident.Literal base.type.Z s) =>
+          match n with
+          | expr.Ident _ (ident.Literal base.type.Z n) =>
+            (Z.eqb s Semantics.width) && is_bounded_by_bool n width_range 
+          | _ => false
+          end
+        | _ => false
+        end
+    | ident.Z_mul_high =>
+      fun args =>
+        let '(s, (x, (y, _))) := args in
+        match s with
+        | expr.Ident _ (ident.Literal base.type.Z s) =>
+          Z.eqb s (2 ^ Semantics.width)
+        | _ => false
+        end
+    | i =>
+      fun _ =>
+        match translate_binop i with
+        | Some x => true
+        | None => false
+        end
+    end.
+
+  Definition valid_cast_exempt_bool {t}
+             (require_in_bounds : bool)
+             (e : @API.expr (fun _ => unit) t) : bool :=
+    match e with
+    | (expr.Ident type_Z (ident.Literal base.type.Z z)) =>
+      if require_in_bounds
+      then is_bounded_by_bool z max_range
+      else true 
+    | (expr.Ident type_nat (ident.Literal base.type.nat n)) =>
+      (* nats are only valid if not required to be in bounds
+         (in practice, this means only if they are an argument to
+         nth_default) *)
+      negb (require_in_bounds)
+    | expr.Var type_listZ x => true
+    | _ => false
+    end.
+
+  Definition valid_cast_bool
+             {t} (f : @API.expr (fun _ => unit) t) : bool :=
+    match f with
+    | expr.App
+        _ _ (expr.Ident _ ident.Z_cast)
+        (expr.Ident type_range (ident.Literal base.type.zrange r)) =>
+      range_good r
+    | expr.App
+        _ _ (expr.Ident _ ident.Z_cast2)
+        (expr.App
+           _ _
+           (expr.App
+              _ _ (expr.Ident _ (ident.pair _ _))
+              (expr.Ident type_range (ident.Literal base.type.zrange r1)))
+           (expr.Ident type_range (ident.Literal base.type.zrange r2))) =>
+      range_good r1 && range_good r2
+    | _ => false
+    end.
+
+  Fixpoint valid_expr_bool {t} (require_cast : bool)
+           (e : @API.expr (fun _ => unit) t) :
+    type.for_each_lhs_of_arrow API.expr t -> bool :=
+    if cast_exempt e
+    then fun _ => valid_cast_exempt_bool require_cast e
+    else if require_cast
+         then match e in expr.expr t0 return
+                    type.for_each_lhs_of_arrow _ t0 -> bool with
+              | expr.App (type.base _) _ f x =>
+                fun y =>
+                  if valid_cast_bool f
+                  then (valid_expr_bool false f (x, y))
+                         && (valid_expr_bool false x tt)
+                  else false
+              | _ => fun _ => false
+              end
+         else
+           match e in expr.expr t0 return
+                 type.for_each_lhs_of_arrow _ t0 -> bool with
+           | expr.App (type.base _) _ f x =>
+             fun y =>
+               let rc := require_cast_for_arg f in
+               (valid_expr_bool false f (x, y))
+                 && (valid_expr_bool rc x tt)
+           | expr.Ident _ i => valid_ident_bool i
+           | expr.Var type_Z x => fun _ => true
+           | expr.Var type_listZ x => fun _ => true
+           | _ => fun _ => false
+           end.
+
+
+  Lemma valid_expr_bool_impl1 {t} (e : API.expr t) :
+    (exists b, t = type.base b) ->
+    forall rc args,
+      valid_expr_bool rc e args = true -> valid_expr rc e.
+  Proof.
+    induction e; intros;
+      cbn [valid_expr_bool cast_exempt negb andb] in *;
+      break_match_hyps;
+      cbn [valid_ident_bool valid_cast_exempt_bool
+                            valid_cast_bool
+                            translate_binop] in *;
+      repeat match goal with
+             | H : false = true |- _ => congruence
+             | H : true = false |- _ => congruence
+             | H : exists _, type.arrow _ _ = type.base _ |- _ =>
+               destruct H; congruence
+             | _ => progress subst
+             | H : _ && _ = true |- _ =>
+               apply andb_true_iff in H; destruct H
+             | H : _ && _ = false |- _ =>
+               apply andb_false_iff in H; destruct H
+             end.
+    { destruct rc;
+        constructor;
+        repeat match goal with
+               | H : is_bounded_by_bool _ _ = true |- _ =>
+                 rewrite H
+               | |- (_ || _)%bool = true => apply Bool.orb_true_iff
+               | _ => tauto
+               end. }
+    { destruct rc;
+        try constructor;
+        repeat match goal with
+               | H : false = true |- _ => congruence
+               | _ => progress cbn [negb] in *
+               | H : is_bounded_by_bool _ _ = true |- _ =>
+                 rewrite H
+               | |- (_ || _)%bool = true => apply Bool.orb_true_iff
+               | _ => tauto
+               end. }
+    { constructor. }
+    { break_match_hyps;
+        try constructor;
+        repeat match goal with
+               | H : false = true |- _ => congruence
+               end. }
+    2:{
+      
+
+
+      cbv [is_cast] in *.
+      break_match_hyps.
+      constructor. 
+  Qed.
+
+  Lemma is_cast_literal_type {var t} (r : @API.expr var t) :
+
+    is_cast_literal r = true ->
+    t = type_range.
+  Proof.
+    cbv [is_cast_literal].
+    break_match; congruence.
+  Qed.
+
+  Lemma valid_cast_ident {var t} (r : @API.expr var t) :
+    is_cast_literal r = true ->
+    (match t as t0 return
+           expr.expr t0 -> Prop with
+     | type_range =>
+       fun r =>
+         r = expr.Ident (ident.Literal (t:=base.type.zrange) max_range)
+     | _ => fun _ => False
+     end) r.
+  Proof.
+    cbv [is_cast_literal].
+    break_match; try congruence.
+    destruct idc.
+
+  Lemma valid_cast_ident {t} (f : API.expr t) :
+    is_cast_ident f = true ->
+    (match t as t0 return
+           expr.expr t0 -> Prop with
+     | type.arrow s1 (type.arrow s2 d) =>
+       fun f =>
+         forall
+           (r : API.expr s1)
+           (x : API.expr s2)
+           (args : type.for_each_lhs_of_arrow API.expr d),
+           is_cast_literal r = true ->
+           valid_expr_bool false (expr.App f r) (x, args) = true ->
+           valid_expr true x ->
+           valid_expr true (expr.App (expr.App f r) x)
+     | _ => fun _ => False
+     end) f.
+  Proof.
+    cbv [is_cast_ident].
+    break_match; try congruence;
+      intros;
+      try match goal with
+          | H: @is_cast_literal _ _ type_range2 _ = true |- _ =>
+            apply is_cast_literal_type in H; congruence
+          end.
+    break_match_hyps; try congruence.
+    apply valid_cast_literal in H0
+    
+
+    2:{
+      intros.
+      apply valid_cast_literal in H0.
+      congruence.
+      exfalso.
+      clear H1.
+      remember type_ZZ.
+      cbv [is_cast_literal] in *.
+      break_match_hyps; try congruence.
+      destruct r; try congruence.
+      destruct idc; try congruence.
+      destruct t; try congruence.
+      { destruct idc0; try congruence.
+        destruct t0; try congruence.
+
+  Lemma valid_cast_impl1 {t} (f : API.expr t):
+    is_cast f = true ->
+    (match t as t0 return expr.expr t0 -> Prop with
+     | type.base _ => fun _ => False
+     | type.arrow s d =>
+       fun f =>
+         forall
+           (x : API.expr s)
+           (args : type.for_each_lhs_of_arrow API.expr d),
+           valid_expr_bool false f (x, args) = true ->
+           (* valid_expr_bool false x tt = true -> *)
+           valid_expr true (expr.App f x)
+     end) f.
+  Proof.
+    cbv [is_cast].
+    break_match; try congruence.
+    remember t.
+    repeat match goal with
+           | |- forall (_: match ?x with | _ => _ end = true), _ =>
+             destruct x; try congruence
+           | |- forall (_: (match ?x with | _ => _ end) _ = true), _ =>
+             destruct x; try congruence
+           | |- forall (_: (match ?x with | _ => _ end) _ _ = true), _ =>
+             destruct x; try congruence
+           end.
+    { break_match.
+      Set Printing Implicit.
+      cbv [is_cast_ident].
+      destruct f1.
+    destruct f; try congruence.
+    destruct s; try congruence.
+    destruct t; try congruence.
+    { destruct t; try congruence. 
+    destruct f1.
+  Lemma is_cast_ident_base
+             {var s d} (e : @API.expr var (s -> d)) :
+    (exists b, d = type.base b) ->
+    is_cast_ident e = false.
+  Proof.
+    cbv [is_cast_ident].
+    destruct e; try reflexivity.
+    destruct idc; try reflexivity.
+    break_match; try congruence. 
+    destruct e; cbn.
+    
+
+
+
+  Definition valid_cast_postcondition {t}
+    : API.expr t -> Prop :=
+    match t as t0 return expr.expr t0 -> Prop with
+     | type.base _ => fun _ => False
+     | type.arrow s d =>
+       fun f =>
+         forall
+           (x : API.expr s)
+           (args : type.for_each_lhs_of_arrow API.expr d),
+           valid_expr_bool false f (x, args) = true ->
+           (* valid_expr_bool false x tt = true -> *)
+           valid_expr true (expr.App f x)
+     end. 
+
+  Lemma valid_cast_apprange {t1 t2}
+        (f : API.expr t1)
+        (r : API.expr t2) :
+    match f with
+    | expr.Ident _ ident.Z_cast =>
+      match r with
+      | expr.Ident _ (ident.Literal base.type.zrange r) =>
+        range_good r
+      | _ => false
+      end
+    | _ => false
+    end = true ->
+    (match t1 as t3 return
+           expr.expr t3 -> expr.expr t2 -> Prop with
+     | type.arrow type_range d =>
+       fun f =>
+         match t2 as t4 return expr.expr t4 -> Prop with
+         | type_range =>
+           fun r =>
+             valid_cast_postcondition (expr.App f r)
+         | _ => fun _ => False
+         end
+     | _ => fun _ _ => False
+     end) f r.
+  Proof.
+    destruct f; try congruence.
+    destruct idc; try congruence.
+    destruct r; try congruence.
+    destruct idc; try congruence.
+    destruct t; try congruence.
+    cbn [valid_cast_postcondition]; intros.
+    cbn [valid_expr_bool cast_exempt require_cast_for_arg] in *.
+    rewrite Bool.andb_false_r in *. congruence.
+  Qed.
+
+  (*
+  Lemma valid_cast2_apppair {t1 t2}
+        (f : API.expr t1)
+        (r : API.expr t2) :
+    match f with
+    | expr.App
+        _ _ (expr.Ident type_range2 (ident.pair _ _))
+        (expr.Ident _ (ident.Literal base.type.zrange r1)))
+        (expr.Ident _ (ident.Literal base.type.zrange r2)) =>
+      range_good r1 && range_good r2
+    | _ => false
+    end
+    | _ => false
+    end = true ->
+    (match t1 as t3 return
+           expr.expr t3 -> expr.expr t2 -> Prop with
+     | type.arrow type_range2 d =>
+       fun f =>
+         match t2 as t4 return expr.expr t4 -> Prop with
+         | type_range2 =>
+           fun r =>
+             valid_cast_postcondition (expr.App f r)
+         | _ => fun _ => False
+         end
+     | _ => fun _ _ => False
+     end) f r.
+  Proof.
+*)
+
+  Lemma of_apprange {var d}
+        (P : forall d,
+            API.expr (var:=var) (type_range -> d) ->
+            API.expr (var:=var) type_range -> Prop)
+        (f : API.expr (type_range -> d))
+        (x : API.expr type_range):
+    (forall t1 t2
+            (f' : API.expr t1)
+            (x' : API.expr t2),
+        (match t1 as t3
+               return expr.expr t3 ->
+                      expr.expr t2 -> Prop with
+         | type.arrow type_range d0 =>
+           fun f'' : API.expr (type_range -> d0) =>
+             match t2 as t4
+                   return expr.expr t4 -> Prop with
+             | type_range =>
+               fun x'' => P d0 f'' x''
+             | _ => fun _ => False
+             end
+         | _ => fun _ _ => False
+         end) f' x') ->
+    P _ f x.
+  Proof.
+    let H := fresh in
+    intro H; specialize (H _ _ f x).
+    assumption.
+  Qed.
+
+  (*
+    match f with
+    | Ident (s -> d) _ => 
+      match x with
+      | _ =>
+      end
+    end = true ->
+    P (f @ x)
+    
+
+
+    match f with
+    | Ident (s -> d) _ => 
+      match x with
+      | _ =>
+      end
+    end = true ->
+    P e
+
+  *)
+  Lemma of_apprange' {var d}
+        (pre : forall t2 t1, (* important to take t2 first *)
+            API.expr (var:=var) t1 ->
+            API.expr (var:=var) t2 -> bool)
+        (P : forall t,
+            API.expr (var:=var) t -> Prop)
+        (f : API.expr (type_range -> d))
+        (x : API.expr type_range):
+    (forall t1 t2 f' x',
+        pre t2 t1 f' x' = true ->
+        (match t1 as t3 return
+               expr.expr t3 -> expr.expr t2 -> Prop with
+         | type.arrow type_range d =>
+           fun f'' =>
+             match t2 as t4 return expr.expr t4 -> Prop with
+             | type_range =>
+               fun x'' =>
+                 P _ (expr.App f'' x'')
+             | _ => fun _ => False
+             end
+         | _ => fun _ _ => False
+         end) f' x') ->
+    (pre _ _ f x = true) ->
+    P d (expr.App f x).
+  Proof.
+    let H := fresh in
+    intro H; specialize (H _ _ f x).
+    assumption.
+  Qed.
+  Lemma of_apprange2 {var d}
+        (pre : forall t2 t1, (* important to take t2 first *)
+            API.expr (var:=var) t1 ->
+            API.expr (var:=var) t2 -> bool)
+        (P : forall t,
+            API.expr (var:=var) t -> Prop)
+        (f : API.expr (type_range2 -> d))
+        (x : API.expr type_range2):
+    (forall t1 t2 f' x',
+        pre t2 t1 f' x' = true ->
+        (match t1 as t3 return
+               expr.expr t3 -> expr.expr t2 -> Prop with
+         | type.arrow type_range2 d =>
+           fun f'' =>
+             match t2 as t4 return expr.expr t4 -> Prop with
+             | type_range2 =>
+               fun x'' =>
+                 P _ (expr.App f'' x'')
+             | _ => fun _ => False
+             end
+         | _ => fun _ _ => False
+         end) f' x') ->
+    (pre _ _ f x = true) ->
+    P d (expr.App f x).
+  Proof.
+    let H := fresh in
+    intro H; specialize (H _ _ f x).
+    assumption.
+  Qed.
+  
+  (*
+  Lemma valid_cast2_apprange {t1 t2}
+        (f : API.expr t1)
+        (r : API.expr t2) :
+    match f with
+    | expr.Ident _ ident.Z_cast2 =>
+      match r with
+      | expr.App
+          _ _ (expr.App
+                 _ _ (expr.Ident type_range2 (ident.pair _ _))
+                 (expr.Ident _ (ident.Literal base.type.zrange r1)))
+          (expr.Ident _ (ident.Literal base.type.zrange r2)) =>
+        range_good r1 && range_good r2
+      | _ => false
+      end
+    | _ => false
+    end = true ->
+    (match t1 as t3 return
+           expr.expr t3 -> expr.expr t2 -> Prop with
+     | type.arrow type_range2 d =>
+       fun f =>
+         match t2 as t4 return expr.expr t4 -> Prop with
+         | type_range2 =>
+           fun r =>
+             valid_cast_postcondition (expr.App f r)
+         | _ => fun _ => False
+         end
+     | _ => fun _ _ => False
+     end) f r.
+  Proof.
+    repeat match goal with
+           | |- forall (_: match ?x with | _ => _ end = true), _ =>
+             destruct x; try congruence
+           | |- forall (_: (match ?x with | _ => _ end) _ = true), _ =>
+             destruct x; try congruence
+           | |- forall (_: (match ?x with | _ => _ end) _ _ = true), _ =>
+             destruct x; try congruence
+           end.
+    eapply of_apprange.
+    destruct r1.
+    destruct f; try congruence.
+    destruct idc; try congruence.
+    destruct r; try congruence.
+    destruct idc; try congruence.
+    destruct t; try congruence.
+    cbn [valid_cast_postcondition]; intros.
+    cbn [valid_expr_bool cast_exempt require_cast_for_arg] in *.
+    rewrite Bool.andb_false_r in *. congruence.
+  Qed.
+*)
+
+  Lemma valid_cast_impl1 {t}
+        (f : API.expr t) :
+    is_cast f = true ->
+    valid_cast_postcondition f.
+  Proof.
+    cbv [is_cast].
+    repeat match goal with
+           | |- forall (_: match ?x with | _ => _ end = true), _ =>
+             destruct x; try congruence
+           | |- forall (_: (match ?x with | _ => _ end) _ = true), _ =>
+             destruct x; try congruence
+           | |- forall (_: (match ?x with | _ => _ end) _ _ = true), _ =>
+             destruct x; try congruence
+           end.
+    { match goal with
+      | e1 : API.expr (type.arrow ?s ?d), e2 : API.expr ?t2
+        |- ?pre = true -> ?Q =>
+        let pre :=
+            lazymatch (eval pattern e2 in pre) with ?f _ => f end in
+        let pre :=
+            lazymatch (eval pattern e1 in pre) with ?f _ => f end in
+        let pre :=
+            lazymatch (eval pattern (type.arrow s d) in pre) with ?f _ => f end in
+        let pre :=
+            lazymatch (eval pattern t2 in pre) with ?f _ => f end in
+        change (pre _ _ e1 e2 = true -> Q);
+          intro;
+          apply (of_apprange' pre); [ | assumption ]
+      end.
+      clear. intros *.
+      repeat match goal with
+             | |- forall (_: match ?x with | _ => _ end = true), _ =>
+               destruct x; try congruence
+             | |- forall (_: (match ?x with | _ => _ end) _ = true), _ =>
+               destruct x; try congruence
+             | |- forall (_: (match ?x with | _ => _ end) _ _ = true), _ =>
+               destruct x; try congruence
+             end.
+      cbn [valid_cast_postcondition]; intros.
+      cbn [valid_expr_bool cast_exempt require_cast_for_arg
+                           valid_ident_bool andb] in *.
+      congruence. }
+    { match goal with
+      | e1 : API.expr (type.arrow ?s ?d), e2 : API.expr ?t2
+        |- ?pre = true -> ?Q =>
+        let pre :=
+            lazymatch (eval pattern e2 in pre) with ?f _ => f end in
+        let pre :=
+            lazymatch (eval pattern e1 in pre) with ?f _ => f end in
+        let pre :=
+            lazymatch (eval pattern (type.arrow s d) in pre) with ?f _ => f end in
+        remember pre end.
+
+      match type of Heqb with _ =
+                              (fun t e (e0 : API.expr type_range2) =>
+                                 ?f) =>
+                              let pre :=
+                                  constr:(fun t t' e (e0 : API.expr t') =>
+                                     f) in
+                              idtac pre
+      end.
+      
+                              idtac f end.
+                              let f := lazymatch (eval pattern type_range2 in x) with ?f _ => f end in idtac f end.
+          idtac t2 pre end.
+        let pre :=
+            lazymatch (eval pattern t2 in pre) with ?f _ => f end in
+          idtac pre end.
+        change (pre _ _ e1 e2 = true -> Q);
+          intro;
+          apply (of_apprange' pre); [ | assumption ]
+      end.
+      clear. intros *.
+      repeat match goal with
+             | |- forall (_: match ?x with | _ => _ end = true), _ =>
+               destruct x; try congruence
+             | |- forall (_: (match ?x with | _ => _ end) _ = true), _ =>
+               destruct x; try congruence
+             | |- forall (_: (match ?x with | _ => _ end) _ _ = true), _ =>
+               destruct x; try congruence
+             end.
+      cbn [valid_cast_postcondition]; intros.
+      cbn [valid_expr_bool cast_exempt require_cast_for_arg
+                           valid_ident_bool andb] in *.
+      congruence. }
+        
+        intros. subst b.
+      pose proof (fun d => @of_apprange' _ d b) as HAPP.
+      intro H.
+      apply HAPP.
+      apply HAPP in H.
+      apply (of_apprange' b).
+      apply H.
+      match goal with
+      | |- ?P -> ?Q =>
+        let pre :=
+            lazymatch (eval pattern f1 in P) with ?f _ => f end in
+        let pre :=
+            lazymatch (eval pattern (type.arrow type_range (type.arrow type_Z type_Z)) in pre) with ?f _ => f end in
+        idtac pre
+      end.
+      
+    (pre _ _ f x = true) ->
+    P d (expr.App f x).
+      eapply of_apprange'; eauto; intros.
+      break_match.
+    { let H := fresh in
+      intro H; apply valid_cast_apprange in H.
+      assumption. }
+    { 
+    destruct f; try congruence.
+    destruct s; try congruence.
+    destruct t; try congruence.
+    { destruct t; try congruence.
+      destruct d; try congruence.
+      destruct d1; try congruence.
+      destruct t; try congruence.
+      destruct t; try congruence.
+      destruct d2; try congruence.
+      destruct t; try congruence.
+      destruct t; try congruence.
+      intros.
+      apply valid_cast_apprange in H.
+      apply H. }
+    { destruct t1; try congruence.
+      destruct t; try congruence.
+      destruct d; try congruence.
+      destruct d1; try congruence.
+      destruct t; try congruence.
+      destruct t; try congruence.
+      destruct d2; try congruence.
+      destruct t; try congruence.
+      destruct t; try congruence.
+      intros.
+      apply valid_cast_apprange in H.
+      apply H. }
+
